reorganisation of pancake related code

HOL/panScript.sml
@@ -2,16 +2,216 @@
  * actual pancake programs
  *)
 
-open stringLib;
-open helperLib;
-open finite_mapTheory; (* flookup_thm *)
+(*/ basic rephrasings
+   not sure whether this should be kept around but lemmas use it atm
+ *)
 
+(* iiter (Ret INL) → Tau (itree_unfold (iiter_cb (mrec_cb h_prog))
+                           (mrec_cb h_prog (⋆ (rh state_res) k))) to continue *)
+(* mrec: Vis (INL (prog × newstate)) k → Ret (INL (h_prog prog ⋆ k)) *)
+(* mrec: Vis (INR (svis_ev × result->itree)) k → Ret (INL (h_prog prog ⋆ k)) *)
+Definition mrec_cb_def[simp]:
+    mrec_cb rh (Ret r) = Ret (INR r)
+  ∧ mrec_cb rh (Tau t) = Ret (INL t)
+  ∧ mrec_cb rh (Vis (INL state_res) k) = Ret (INL (⋆ (rh state_res) k))
+  ∧ mrec_cb rh (Vis (INR   ffi_res) k) = Vis ffi_res (λx. Ret (INL (k x)))
+End
+
+Theorem itree_mrec_alt:
+  itree_mrec rh seed = mrec_cb rh ↻ rh seed
+Proof
+  rw[itree_mrec_def] >>
+  AP_THM_TAC >>
+  AP_TERM_TAC >>
+  rw[FUN_EQ_THM] >>
+  rw[DefnBase.one_line_ify NONE mrec_cb_def]
+QED
+
+(* Dec cleanup *)
+
+Definition revert_binding_def:
+  revert_binding name old_s
+  = (λ(res,s').
+       Ret
+       (res,
+        s' with locals :=
+        res_var s'.locals (name,FLOOKUP old_s.locals name)))
+End
+
+Theorem h_prog_rule_dec_alt:
+  h_prog_rule_dec vname e p s =
+  case eval s e of
+    NONE => Ret (SOME Error,s)
+  | SOME value =>
+      Vis (INL (p,s with locals := s.locals |+ (vname,value)))
+          (revert_binding vname s)
+Proof
+  rw[h_prog_rule_dec_def, revert_binding_def]
+QED
+
+(* (* f, f' type vars instantiated differently smh *) *)
+(* Theorem mrec_bind_lemma: *)
+(*   ∀f f'. *)
+(*   (∀a. ∃r. (f a) = (Ret r) ∧ (f' a) = (Ret r)) ⇒ *)
+(*   ∀t. (mrec_cb h_prog) ↻ (⋆ t f) = *)
+(*       (⋆ (mrec_cb h_prog ↻ t) f') *)
+(* Proof *)
+(*   rpt strip_tac >> *)
+(*   qspecl_then [‘(mrec_cb h_prog) ↻ (⋆ t f)’, *)
+(*                ‘⋆ (mrec_cb h_prog ↻ t) f'’] *)
+(*               strip_assume_tac itree_bisimulation >> *)
+(*   fs[EQ_IMP_THM] >> *)
+(*   qpat_x_assum ‘_ ⇒ ∃R. _’ kall_tac >> *)
+(*   pop_assum irule >> *)
+(*   qexists_tac ‘λa b. ∃t name s. *)
+(*                 a = (mrec_cb h_prog ↻ (⋆ t f)) ∧ *)
+(*                 b = (⋆ (mrec_cb h_prog ↻ t) f')’ >> *)
+(*   rw[] >- *)
+(*    metis_tac[] >- (* base case *) *)
+(*    (* ret *) *)
+(*    (Cases_on ‘t'’ >- *)
+(*      (fs[Once itree_iter_thm, itree_bind_thm] >> *)
+(*       last_assum $ qspec_then ‘x'’ strip_assume_tac >> *)
+(*       fs[itree_bind_thm]) >- *)
+(*      (fs[Once itree_iter_thm, itree_bind_thm]) >- *)
+(*      (Cases_on ‘a’ >- *)
+(*        fs[Once itree_iter_thm, itree_bind_thm] >- *)
+(*        fs[Once itree_iter_thm, itree_bind_thm])) >- *)
+(*    (* tau *) *)
+(*    (Cases_on ‘t'’ >- *)
+(*      (fs[Once itree_iter_thm, itree_bind_thm] >> *)
+(*       last_assum $ qspec_then ‘x’ strip_assume_tac >> *)
+(*       fs[itree_bind_thm]) >- *)
+(*      (fs[Once itree_iter_thm, itree_bind_thm] >> *)
+(*       metis_tac[]) >- *)
+(*      (Cases_on ‘a’ >- *)
+(*        (fs[Once itree_iter_thm, itree_bind_thm] >> *)
+(*         metis_tac[itree_bind_assoc]) >- *)
+(*        fs[Once itree_iter_thm, itree_bind_thm])) >- *)
+(*    (* vis *) *)
+(*    (Cases_on ‘t'’ >- *)
+(*      (fs[Once itree_iter_thm, itree_bind_thm] >> *)
+(*       last_assum $ qspec_then ‘x’ strip_assume_tac >> *)
+(*       fs[itree_bind_thm]) >- *)
+(*      fs[Once itree_iter_thm, itree_bind_thm] >- *)
+(*      (Cases_on ‘a'’ >- *)
+(*        fs[Once itree_iter_thm, itree_bind_thm] >- *)
+(*        (fs[Once itree_iter_thm, itree_bind_thm] >> *)
+(*         strip_tac >> *)
+(*         (* stuck on extra Tau from iter on (Ret INL) from (Vis INR) *) *)
+(*        ))) *)
+(* QED *)
+
+(* relies on mrec_cb h_prog rev -> only Ret INR, so can't prolong iteration *)
+(* also applies to while and cond! *)
+Theorem dec_lemma:
+  ∀ t name s.
+    ≈ (mrec_cb h_prog ↻ (⋆ t (revert_binding name s)))
+      (⋆ (mrec_cb h_prog ↻ t) (revert_binding name s))
+Proof
+  qspecl_then
+  [‘λa b. ∃t name s.
+     a = (mrec_cb h_prog ↻ (⋆ t (revert_binding name s))) ∧
+     b = (⋆ (mrec_cb h_prog ↻ t) (revert_binding name s))’]
+  strip_assume_tac itree_wbisim_strong_coind >>
+  rpt strip_tac >>
+  pop_assum irule >>
+  rw[] >-
+   (Cases_on ‘t''’ >-
+     (or3_tac >> (* Ret produces Ret, doesn't affect iter. easy! *)
+      Cases_on ‘x’ >>
+      rw[revert_binding_def] >>
+      rw[Once itree_iter_thm, itree_bind_thm] >>
+      rw[Once itree_iter_thm, itree_bind_thm]) >-
+     (* Tau case is clear *)
+     (or1_tac >>
+      rw[Once itree_iter_thm, itree_bind_thm] >>
+      rw[Once itree_iter_thm, itree_bind_thm] >>
+      metis_tac[]) >-
+     (* Vis case is a bit tricky, depends on whether the event is silent *)
+     (Cases_on ‘a’ >-
+       (or1_tac >>
+        rw[Once itree_iter_thm, itree_bind_thm] >>
+        rw[Once itree_iter_thm, itree_bind_thm] >>
+        metis_tac[itree_bind_assoc]) >-
+       (or2_tac >>
+        rw[Once itree_iter_thm, itree_bind_thm] >>
+        rw[Once itree_iter_thm, itree_bind_thm] >>
+        or1_tac >>
+        qexistsl_tac [‘Tau (g r)’, ‘name’, ‘s’] >>
+        CONJ_TAC >-
+         (CONV_TAC $ RHS_CONV $ ONCE_REWRITE_CONV[itree_bind_thm] >>
+          CONV_TAC $ RHS_CONV $ ONCE_REWRITE_CONV[itree_iter_thm] >>
+          rw[itree_bind_thm]) >-
+         (CONV_TAC $ RHS_CONV $ ONCE_REWRITE_CONV[itree_iter_thm] >>
+          rw[itree_bind_thm])))) >-
+   metis_tac[]
+QED
+
+Theorem dec_thm:
+  (eval s e = SOME k) ⇒
+  ≈ (itree_mrec h_prog (Dec name e p,s))
+    (⋆
+     (itree_mrec h_prog (p,s with locals := s.locals |+ (name,k)))
+     (revert_binding name s))
+Proof
+  rw[itree_mrec_alt] >>
+  rw[h_prog_def, h_prog_rule_dec_def] >>
+  rw[Once itree_iter_thm, itree_bind_thm] >>
+  rw[GSYM revert_binding_def] >>
+  metis_tac[dec_lemma, itree_wbisim_tau_eq, itree_wbisim_trans]
+QED
+
+(*/ massaging into ffi itree
+   TODO change when fixed, also prove it respects wbisim or have a bad time
+ *)
+
+Definition massage_cb_def[simp]:
+    massage_cb (INL (Ret (res,s))) = Ret' res
+  ∧ massage_cb (INR (Ret (res,s))) = Ret' res
+  ∧ massage_cb (INL (Tau t)) = Tau' (INL t)
+  ∧ massage_cb (INR (Tau t)) = Tau' (INR t)
+  ∧ massage_cb (INL (Vis (e,k) g)) = Vis' e (λr. INR (k r))
+  ∧ massage_cb (INR (Vis e g))     = Vis' e (INR ∘ g)
+End
+
+(* massage Ret type from (η x state) -> η *)
+(* convert Vis (sem_vis_event x (FFI_result -> itree)) ((prog x state) -> %itree)
+-> Vis sem_vis_event (FFI_result -> itree) *)
+Definition massage_def:
+  massage x = itree_unfold massage_cb (INL x)
+End
+
+Theorem massage_thm:
+    massage (Ret (res, s)) = Ret res ∧ massage (Tau t) = Tau (massage t)
+Proof
+  rw[massage_def] >-
+   rw[Once itree_unfold] >-
+   (rw[Once itree_unfold] >> rw[GSYM massage_def])
+QED
+
+Theorem itree_evaluate_alt:
+  itree_evaluate p s = massage (itree_mrec h_prog (p,s))
+Proof
+  rw[itree_evaluate_def, massage_def] >>
+  AP_THM_TAC >> (* same fn => same on same arg, backwards *)
+  AP_TERM_TAC >>
+  rw[FUN_EQ_THM] >>
+  rw[DefnBase.one_line_ify NONE massage_cb_def]
+QED
+
+(* hol imports *)
+open finite_mapTheory; (* FLOOKUP_UPDATE *)
+open helperLib; (* remove_whitespace *)
+open stringLib; (* fromMLstring... *)
+(* open wordsTheory; (* n2w_def *) *)
+
+(* cakeml imports *)
 open asmTheory; (* word_cmp_def *)
 open miscTheory; (* read_bytearray *)
 open panLangTheory; (* size_of_shape_def *)
 open panPtreeConversionTheory; (* parse_funs_to_ast *)
 open wordLangTheory; (* word_op_def *)
-open wordsTheory; (* n2w_def *)
 
 local
   val f =
@@ -131,18 +331,20 @@ Proof
   rw[Once itree_iter_thm, itree_bind_thm] >>
   (* while *)
   rw[Once h_prog_def, h_prog_rule_while_alt] >>
-  rw[Once itree_iter_thm] >>
-  rw[Once itree_iter_thm] >>
-  rw[eval_def, FLOOKUP_UPDATE, word_cmp_def, cheat1] >>
+  rw[Once itree_iter_thm] >> rw[Once itree_iter_thm] >>
+  rw[Once eval_def] >> rw[Once eval_def] >>
+  rw[FLOOKUP_UPDATE] >>
+  rw[Once eval_def, word_cmp_def, cheat1] >>
   rw[itree_bind_thm] >>
   (* assignment *)
   rw[Once h_prog_def, h_prog_rule_assign_def] >>
-  rw[eval_def, FLOOKUP_UPDATE, cheat1,
-     word_op_def, is_valid_value_def, shape_of_def] >>
+  rw[Once eval_def] >> rw[Once eval_def] >>
+  rw[FLOOKUP_UPDATE, word_op_def, is_valid_value_def, shape_of_def,
+     Once eval_def, cheat1] >>
   rw[Once itree_iter_thm, itree_bind_thm] >>
   (* second while *)
-  rw[Once itree_iter_thm] >>
-  rw[Once itree_iter_thm] >>
+  (* rw[GSYM h_prog_rule_while_alt, GSYM h_prog_def] *)
+  rw[Once itree_iter_thm] >> rw[Once itree_iter_thm] >>
   rw[eval_def, FLOOKUP_UPDATE, word_cmp_def] >>
   rw[revert_binding_def] >>
   rw[Once itree_iter_thm, itree_bind_thm] >>
